$$
    r_{TE} \equiv \left( \frac{E_{ro}}{E_{io}} \right)_{TE} = \left( \frac{E_r}{E_i} \right)_{TE} = \frac{n_i \cos\theta_i - n_t \cos\theta_t}{n_i \cos\theta_i + n_t \cos\theta_t}
    \tag{8-24}
$$$$
    t_{TE} \equiv \left( \frac{E_{to}}{E_{io}} \right)_{TE} = \left( \frac{E_t}{E_i} \right)_{TE} = \frac{2 n_i \cos\theta_i}{n_i \cos\theta_i + n_t \cos\theta_t}
    \tag{8-25}
$$$$
    r_{TM} \equiv \left( \frac{E_{ro}}{E_{io}} \right)_{TM} = \left( \frac{E_r}{E_i} \right)_{TM} = \frac{-n_t \cos\theta_i + n_i \cos\theta_t}{n_t \cos\theta_i + n_i \cos\theta_t}
    \tag{8-26}
$$$$
    t_{TM} \equiv \left( \frac{E_{to}}{E_{io}} \right)_{TM} = \left( \frac{E_t}{E_i} \right)_{TM} = \frac{2 n_i \cos\theta_i}{n_t \cos\theta_i + n_i \cos\theta_t}
    \tag{8-27}
$$
